firmware/IncrementWait/Incr.v
@@ -1,0 +1,528 @@
+Require Import Coq.Lists.List.
+Require Import Coq.micromega.Lia.
+Require Import Coq.ZArith.ZArith.
+
+Require Import Cava.Expr.
+Require Import Cava.ExprProperties.
+Require Import Cava.Invariant.
+Require Import Cava.Primitives.
+Require Import Cava.Semantics.
+Require Import Cava.TLUL.
+Require Import Cava.Types.
+Require Import Cava.Util.BitArithmetic.
+Require Import Cava.Util.List.
+Require Import Cava.Util.Tactics.
+
+Require Import coqutil.Tactics.Simp.
+Require Import coqutil.Tactics.Tactics.
+
+Import ListNotations.
+
+Section Var.
+  Import Expr.
+  Import ExprNotations.
+  Import PrimitiveNotations.
+
+  Local Open Scope N.
+
+  Context {var : tvar}.
+
+  Definition incr_state := BitVec 2.
+  Definition Idle       := Constant incr_state 0.
+  Definition Busy1      := Constant incr_state 1.
+  Definition Busy2      := Constant incr_state 2.
+  Definition Done       := Constant incr_state 3.
+
+  Definition inner
+    : Circuit _ [Bit; BitVec 32] (Bit ** BitVec 32)
+    := {{
+      fun valid data =>
+        let/delay '(istate; value) :=
+           let istate' :=
+               if istate == `Busy1` then `Busy2`
+               else if istate == `Busy2` then `Done`
+                    else if istate == `Done` then `Idle`
+                         else (* istate == `Idle` *)
+                           if valid then `Busy1`
+                           else `Idle` in
+
+           let value' :=
+               if istate == `Busy2` then value + `K 1`
+               else if istate == `Idle` then data
+                    else value in
+
+           (istate', value')
+             initially default
+           : denote_type (incr_state ** BitVec 32)
+        in
+        (istate == `Done`, value)
+       }}.
+
+  Definition incr
+    : Circuit _ [tl_h2d_t] tl_d2h_t
+    := {{
+      fun tl_h2d =>
+        (* Destruct and reassemble tl_h2d with a_address that matches the
+           tlul_adapter_reg interface. *)
+        let '(a_valid
+              , a_opcode
+              , a_param
+              , a_size
+              , a_source
+              , a_address
+              , a_mask
+              , a_data
+              , a_user
+              ; d_ready) := tl_h2d in
+        (* Bit #2 of the address determines which register is being accessed *)
+        (*    (STATUS or VALUE). Zero out the other bits. *)
+        let a_address := a_address & (`K 1` << 2) in
+        let tl_h2d := (a_valid
+                       , a_opcode
+                       , a_param
+                       , a_size
+                       , a_source
+                       , a_address
+                       , a_mask
+                       , a_data
+                       , a_user
+                       , d_ready) in
+
+        let/delay '(busy, done, registers; tl_d2h) :=
+           let '(tl_d2h'; req) := `tlul_adapter_reg` tl_h2d registers in
+           let '(is_read, is_write, address, write_data; _write_mask) := req in
+
+           let '(inner_res_valid; inner_res) := `inner` (!busy && !done && is_write) write_data in
+
+           let busy' :=
+               if busy then !inner_res_valid
+               else !done && is_write in
+
+           let done' :=
+               if busy then inner_res_valid
+               else if done then !(is_read && address == `K 0`)
+                    else done in
+
+           let registers' :=
+               if inner_res_valid then `replace` registers `K (sz:=1) 0` inner_res
+               else registers in
+
+           let registers' :=
+               if busy' then `replace` registers' `K (sz:=1) 1` `K 2`
+               else if done' then `replace` registers' `K (sz:=1) 1` `K 4`
+                    else `replace` registers' `K (sz:=1) 1` `K 1` in
+
+           (busy', done', registers', tl_d2h') initially
+           (false, (false, ([0; 1], set_a_ready true (default (t:=tl_d2h_t)))))
+           : denote_type (Bit ** Bit ** Vec (BitVec 32) 2 ** tl_d2h_t)
+        in
+
+        tl_d2h
+       }}.
+End Var.
+
+Definition sim {s i o} (c : Circuit s i o) (input : list (denote_type i))
+  : list (denote_type s * denote_type i * denote_type o) :=
+  fst (List.fold_left (fun '(acc, s) i =>
+                         let '(s', o) := step c s i in
+                         (acc ++ [(s, i, o)], s'))
+                      input
+                      ([], reset_state c)).
+
+Example sample_trace :=
+  Eval compute in
+    let nop := set_d_ready true tl_h2d_default in
+    let read_reg (r : N) :=
+        set_a_valid true
+        (set_a_opcode Get
+        (set_a_size 2%N
+        (set_a_address r
+        (set_d_ready true tl_h2d_default)))) in
+    let write_val (v : N) :=
+        set_a_valid true
+        (set_a_opcode PutFullData
+        (set_a_size 2%N
+        (set_a_address 0%N (* value-ref *)
+        (set_a_data v
+        (set_d_ready true tl_h2d_default))))) in
+
+    sim incr
+        [ (nop, tt)
+          ; (read_reg 4, tt) (* status *)
+          ; (nop, tt)
+          ; (write_val 42, tt)
+          ; (nop, tt)
+          ; (nop, tt)
+          ; (read_reg 4, tt) (* status *)
+          ; (nop, tt)
+          ; (read_reg 0, tt) (* value *)
+          ; (nop, tt)
+          ; (read_reg 4, tt) (* status *)
+        ]%N.
+(* Print sample_trace. *)
+
+Section Spec.
+  Local Open Scope N.
+
+  Variant repr_state :=
+  | ReprIdle
+  | ReprBusy (data : N) (count : nat)
+  | ReprDone (res : N).
+
+  Notation inner_repr := repr_state.
+
+  Global Instance inner_invariant : invariant_for inner inner_repr :=
+    fun (state : denote_type (state_of inner)) repr =>
+      let '(istate, value) := state in
+      match repr with
+      | ReprIdle => istate = 0
+      | ReprBusy data c => (0 < c <= 2)%nat /\ istate = N.of_nat c /\ value = data
+      | ReprDone res => istate = 3 /\ value = res
+      end.
+
+  Definition inner_spec_step (input : denote_type (input_of inner)) repr :=
+    let '(valid, (data, tt)) := input in
+    match repr with
+    | ReprIdle => if valid then ReprBusy data 1 else ReprIdle
+    | ReprBusy data 2 => ReprDone ((data + 1) mod 2^32)
+    | ReprBusy data c => ReprBusy data (c + 1)
+    | ReprDone _ => ReprIdle
+    end.
+
+  Instance inner_specification
+    : specification_for inner inner_repr :=
+    {| reset_repr := ReprIdle;
+
+       update_repr :=
+         fun (input : denote_type (input_of inner)) repr =>
+           inner_spec_step input repr;
+
+       precondition :=
+         fun (input : denote_type (input_of inner)) repr => True;
+
+       postcondition :=
+         fun (input : denote_type (input_of inner)) repr
+           (output : denote_type (output_of inner)) =>
+           let repr' := inner_spec_step input repr in
+           match repr' with
+           | ReprDone res => output = (true, res)
+           | _ => exists res, output = (false, res)
+           end;
+    |}.
+
+  Lemma inner_invariant_at_reset : invariant_at_reset inner.
+  Proof.
+    simplify_invariant inner. reflexivity.
+  Qed.
+
+  Lemma inner_invariant_preserved : invariant_preserved inner.
+  Proof.
+    intros (valid, (data, t)) state repr. destruct t.
+    cbn in * |-. destruct state as (istate, value).
+    intros repr' ? Hinvar Hprec; subst.
+    simplify_invariant inner.
+    simplify_spec inner.
+    cbv [inner inner_spec_step]. stepsimpl.
+    repeat (destruct_pair_let; cbn [fst snd]).
+    destruct repr as [|? iiscount|?]; logical_simplify; subst.
+    - destruct valid; cbn; ssplit; lia.
+    - destruct iiscount as [|[|[|iiscount]]]; cbn; ssplit; lia.
+    - reflexivity.
+  Qed.
+
+  Lemma inner_output_correct : output_correct inner.
+  Proof.
+    intros (valid, (data, t)) state repr. destruct t.
+    cbn in * |-. destruct state as (istate, value).
+    remember (update_repr (c:=inner) (valid, (data, tt)) repr) as repr'.
+    intros Hinvar Hprec.
+    simplify_invariant inner.
+    simplify_spec inner.
+    cbv [inner inner_spec_step]. stepsimpl.
+    repeat (destruct_pair_let; cbn [fst snd]).
+    destruct repr as [|? iiscount|?]; logical_simplify; subst.
+    - destruct valid; eexists; cbn; ssplit; reflexivity.
+    - destruct iiscount as [|[|[|iiscount]]]; try lia; eexists; reflexivity.
+    - eexists. reflexivity.
+  Qed.
+
+  Existing Instances inner_invariant_at_reset inner_invariant_preserved
+           inner_output_correct.
+  Global Instance inner_correctness : correctness_for inner.
+  Proof. constructor; typeclasses eauto. Defined.
+
+  Definition repr := (repr_state * list N * TLUL.repr_state * inner_repr)%type.
+
+  Global Instance incr_invariant : invariant_for incr repr :=
+    fun (state : denote_type (state_of incr)) repr =>
+      let '((s_busy, (s_done, (s_regs, s_d2h))), (s_tlul, s_inner)) := state in
+      let '(r_state, r_regs, r_tl, r_inner) := repr in
+      tlul_invariant (reg_count:=2) s_tlul r_tl
+      /\ match r_tl with
+        | TLUL.Idle =>
+          d_valid    s_d2h = false
+          /\ d_error  s_d2h = false
+          /\ a_ready  s_d2h = true
+        | TLUL.OutstandingAccessAckData h2d regs =>
+          d_valid    s_d2h = true
+          /\ d_opcode s_d2h = AccessAckData
+          /\ d_param  s_d2h = 0
+          /\ d_size   s_d2h = (a_size h2d)
+          /\ d_source s_d2h = (a_source h2d)
+          /\ d_sink   s_d2h = 0
+          /\ d_data   s_d2h = (List.nth (N.to_nat ((((a_address h2d) / 4) mod (2 ^ 30)))) regs 0%N)
+          /\ d_user   s_d2h = 0
+          /\ d_error  s_d2h = false
+          /\ a_ready  s_d2h = false
+        | TLUL.OutstandingAccessAck h2d  =>
+          d_valid    s_d2h = true
+          /\ d_opcode s_d2h = AccessAck
+          /\ d_param  s_d2h = 0
+          (* /\ d_size   s_d2h =  *)
+          /\ d_source s_d2h = (a_source h2d)
+          /\ d_sink   s_d2h = 0
+          /\ d_user   s_d2h = 0
+          /\ d_error  s_d2h = false
+          /\ a_ready  s_d2h = false
+        end
+      /\ inner_invariant s_inner r_inner
+      /\ match r_state with
+        | ReprIdle => s_busy = false /\ s_done = false
+                     /\ r_inner = ReprIdle
+                     /\ nth 1 r_regs 0%N = 1
+        | ReprBusy data count => s_busy = true /\ s_done = false
+                                /\ r_inner = ReprBusy data count
+                                /\ nth 1 r_regs 0%N = 2
+        | ReprDone res => s_busy = false /\ s_done = true
+                         /\ (r_inner = ReprDone res \/ r_inner = ReprIdle)
+                         /\ nth 0 r_regs 0%N = res
+                         /\ nth 1 r_regs 0%N = 4
+        end
+      /\ s_regs = r_regs
+      /\ length r_regs = 2%nat.
+
+  Existing Instance tl_specification.
+
+  Instance incr_specification
+    : specification_for incr repr :=
+    {| reset_repr := (ReprIdle, [0; 1], TLUL.Idle, ReprIdle);
+
+       update_repr :=
+         fun (input : denote_type (input_of incr)) repr =>
+           let '(i_h2d, tt) := input in
+           let '(r_state, r_regs, r_tl, r_inner) := repr in
+
+           let h2d := set_a_address (N.land (a_address i_h2d) 4) i_h2d in
+
+           let r_tl' :=
+               let tlul_input := (h2d, (r_regs, tt)) in
+               update_repr (c:=tlul_adapter_reg (reg_count:=2))
+                           tlul_input r_tl in
+
+           (* compute (some) tlul output *)
+           let '(is_read, is_write, address, write_data) :=
+               match r_tl' with
+               | TLUL.Idle => (false, false, 0, 0)
+               | TLUL.OutstandingAccessAckData _ _ =>
+                 match r_tl with
+                   | TLUL.Idle => (a_valid h2d, false, a_address h2d, 0)
+                   | _ => (false, false, 0, 0)
+                 end
+               | TLUL.OutstandingAccessAck _ =>
+                 match r_tl with
+                 | TLUL.Idle => (false, a_valid h2d, a_address h2d, a_data h2d)
+                 | _ => (false, false, 0, 0)
+                 end
+               end in
+
+           let r_inner' :=
+               let inner_input := (match r_state with ReprIdle => is_write | _ => false end,
+                                   (write_data, tt)) in
+               update_repr (c:=inner) inner_input r_inner in
+
+           let r_state' :=
+               match r_state with
+               | ReprDone _ =>
+                   if (is_read && (address =? 0))%bool then ReprIdle
+                   else r_state
+               | _ =>
+                 match r_inner' with
+                 | ReprBusy data count => ReprBusy data count
+                 | ReprDone res => ReprDone res
+                 | _ => r_state
+                 end
+               end in
+
+           let r_regs' :=
+               match r_inner' with
+               | ReprDone res => replace 0 res r_regs
+               | _ => r_regs
+               end in
+
+           let r_regs' :=
+               match r_state' with
+               | ReprIdle => replace 1 1 r_regs'
+               | ReprBusy _ _ => replace 1 2 r_regs'
+               | ReprDone _ => replace 1 4 r_regs'
+               end in
+
+           (r_state', r_regs', r_tl', r_inner');
+
+       precondition :=
+         fun (input : denote_type (input_of incr)) repr =>
+           let '(i_h2d, tt) := input in
+           let '(r_state, r_regs, r_tl, r_inner) := repr in
+
+           let h2d := set_a_address (N.land (a_address i_h2d) 4) i_h2d in
+
+           let tlul_input := (h2d, (r_regs, tt)) in
+
+           let prec_tlul :=
+               precondition (tlul_adapter_reg (reg_count:=2))
+                            tlul_input r_tl in
+
+           let prec_inner :=
+               forall d2h is_read is_write address write_data write_mask,
+                 postcondition (tlul_adapter_reg (reg_count:=2))
+                               tlul_input r_tl
+                               (d2h, (is_read, (is_write, (address, (write_data, write_mask)))))
+                 -> precondition inner (match r_state with ReprIdle => is_write | _ => false end,
+                                       (write_data, tt)) r_inner in
+
+           prec_tlul /\ prec_inner;
+
+       postcondition :=
+         fun (input : denote_type (input_of incr)) repr
+           (output : denote_type (output_of incr)) =>
+           let '(i_h2d, tt) := input in
+           let '(r_state, r_regs, r_tl, r_inner) := repr in
+           let h2d := set_a_address (N.land (a_address i_h2d) 4) i_h2d in
+
+           (* let postc_tlul := *)
+           (*     let tlul_input := (h2d, (r_regs, tt)) in *)
+           (*     exists req, *)
+           (*       postcondition (tlul_adapter_reg (reg_count:=2)) *)
+           (*                     tlul_input r_tl *)
+           (*                     (output, req) in *)
+           (* postc_tlul; *)
+           True;
+    |}.
+
+  Lemma incr_invariant_at_reset : invariant_at_reset incr.
+  Proof.
+    simplify_invariant incr.
+    cbn. ssplit; [apply (tlul_adapter_reg_invariant_at_reset (reg_count:=2))
+                 |reflexivity..].
+  Qed.
+
+  Existing Instance tlul_adapter_reg_correctness.
+
+  Lemma incr_invariant_preserved : invariant_preserved incr.
+  Proof.
+    intros (h2d, t) state (((r_state, r_regs), r_tl), r_inner). destruct t.
+    cbn in * |-. destruct state as ((busy, (done, (registers, d2h))), (tl_st, inner_st)).
+    destruct_tl_h2d. destruct_tl_d2h.
+    intros repr' ? Hinvar Hprec; subst.
+    simplify_invariant incr. logical_simplify. subst.
+    simplify_spec incr. logical_simplify. subst.
+    (* destruct Hprec as [regs Hprec]. *)
+    match goal with
+    | |- context [step incr ?s ?i] =>
+      remember (step incr s i) as step eqn:Estep;
+        cbv -[Semantics.step inner tlul_adapter_reg] in Estep;
+          subst
+    end.
+    stepsimpl.
+    use_correctness.
+    clear H5.
+    rename H9 into Hpostc_tl.
+    repeat (destruct_pair_let; cbn [fst snd]).
+    ssplit.
+    - eapply tlul_adapter_reg_invariant_preserved.
+      2: apply H.
+      + reflexivity.
+      + assumption.
+    - pose (r_tl_:=r_tl); destruct r_tl; logical_simplify; subst.
+      + destruct_tl_h2d; destruct_tl_d2h; tlsimpl; subst.
+        pose (r_state_:=r_state); destruct r_state; cbn in *; logical_simplify; subst;
+          pose (a_valid_:=a_valid); (destruct a_valid;
+                                     [ match goal with
+                                       | H: true = true -> _ |- _ =>
+                                         destruct H; [auto|subst..]
+                                       end|]); cbn in *; logical_simplify; subst;
+            ssplit; auto.
+      + destruct_tl_h2d; destruct_tl_d2h; tlsimpl; subst.
+        pose (r_state_:=r_state); destruct r_state; cbn in *; logical_simplify; subst;
+          pose (d_ready_:=d_ready); destruct d_ready; cbn in *; logical_simplify; subst;
+            ssplit; auto.
+      + destruct_tl_h2d; destruct_tl_d2h; tlsimpl; subst.
+        pose (r_state_:=r_state); destruct r_state; cbn in *; logical_simplify; subst;
+          pose (d_ready_:=d_ready); destruct d_ready; cbn in *; logical_simplify; subst;
+            ssplit; reflexivity.
+    - eapply inner_invariant_preserved.
+      2: eassumption.
+      + simpl in *.
+        destruct r_inner; try reflexivity.
+        destruct r_tl eqn:Houts; logical_simplify; subst.
+        * destruct a_valid eqn:Hvalid; logical_simplify; subst.
+          -- match goal with
+             | H: true = true -> _ |- _ =>
+               destruct H; try reflexivity; subst
+             end; logical_simplify; subst;
+               boolsimpl; destruct r_state; logical_simplify; subst;
+                 cbn in Hpostc_tl |- *; logical_simplify; subst; reflexivity.
+          -- boolsimpl; destruct r_state; reflexivity.
+
+        * destruct d_ready; logical_simplify; subst;
+            boolsimpl; destruct r_state; reflexivity.
+        * destruct d_ready; logical_simplify; subst;
+            boolsimpl; destruct r_state; reflexivity.
+      + simplify_spec inner. auto.
+    - destruct r_tl; destruct r_inner; destruct r_state; destruct inner_st;
+        logical_simplify; subst; simplify_invariant inner; try discriminate.
+      all: simplify_spec (tlul_adapter_reg (reg_count:=2)); logical_simplify; tlsimpl; subst.
+      all: destruct a_valid; [destruct H3; subst|]; cbn in Hpostc_tl; logical_simplify; subst; cbn.
+      all: eauto.
+      all: destruct_tl_d2h; tlsimpl; subst.
+      all: try (destruct (N.land a_address 4 =? 0) eqn:Haddr;
+               ssplit; eauto;
+               destruct x0 as [|? [|]]; cbn in *; try discriminate; reflexivity).
+      all: try (destruct count as [|[|[|]]]; [lia|..|lia]; cbn;
+             ssplit; eauto;
+             destruct x0 as [|? [|]]; cbn in *; try discriminate; reflexivity).
+      all: try (destruct H6; discriminate).
+      all: try (destruct d_ready; logical_simplify; subst; cbn;
+                  ssplit; eauto;
+                  destruct x0 as [|? [|]]; cbn in *; try discriminate; reflexivity).
+    - destruct r_tl; destruct r_inner; destruct r_state; destruct inner_st;
+        logical_simplify; subst.
+      all: simplify_invariant inner.
+      all: try discriminate.
+      all: simplify_spec (tlul_adapter_reg (reg_count:=2)); logical_simplify; tlsimpl; subst.
+      all: destruct a_valid; [destruct H3; subst|]; cbn in Hpostc_tl; logical_simplify; subst; cbn.
+      all: eauto.
+      all: try (destruct (N.land a_address 4 =? 0) eqn:Haddr;
+               ssplit; eauto;
+               destruct x0 as [|? [|]]; cbn in *; try discriminate; reflexivity).
+      all: try (destruct count as [|[|[|]]]; [lia|..|lia]; cbn;
+             ssplit; eauto;
+             destruct x0 as [|? [|]]; cbn in *; try discriminate; reflexivity).
+      all: try (destruct H6; discriminate).
+      all: try (destruct d_ready; logical_simplify; subst; cbn;
+                  ssplit; eauto;
+                  destruct x0 as [|? [|]]; cbn in *; try discriminate; reflexivity).
+    - repeat destruct_one_match; rewrite ! length_replace; assumption.
+  Qed.
+
+  Lemma incr_output_correct : output_correct incr.
+  Proof.
+    intros ? **.
+    simplify_spec incr. destruct input. destruct d0. destruct r as [[[? ?] ?] ?].
+    apply I.
+  Qed.
+
+  Existing Instances incr_invariant_at_reset incr_invariant_preserved
+           incr_output_correct.
+  Global Instance incr_correctness : correctness_for incr.
+  Proof. constructor; typeclasses eauto. Defined.
+End Spec.
